theories/Core/Completeness/VariableCases.v
@@ -6,20 +6,47 @@ From McPTS.Core.Completeness Require Import LogicalRelation.
 From McPTS.Core.Syntactic Require Import SystemOpt.
 Import Domain_Notations.
 
-Lemma valid_lookup {P : PtsSig} {pred_P : PredicativeSig P} : forall {Γ x A env_relΓ}
-                        (equiv_Γ_Γ : {{ EF Γ ≈ Γ ∈ per_ctx_env pred_P ↘ env_relΓ }}),
+(** ** Cases for global variables *)
+Lemma valid_exp_gvar {P} {pred_P : PredicativeSig P} : forall {Δ Γ σ A x},
+    {{ ⟪ pred_P ⟫ Δ ▶ Γ ⊨s σ : ⋅ }} ->
+    {{ `#x : A ∈ Δ }} ->
+    {{ ⟪ pred_P ⟫ Δ ▶ Γ ⊨u `#x : A[σ] }}.
+Proof.
+  intros * [env_relΓ [? [env_rel []]]] HxinΔ.
+  eexists_rel_exp.
+  assert (rel_sub Δ σ ρ σ ρ' env_rel) as [] by mauto 2.
+  split.
+  - econstructor.
+    econstructor; mauto 2.
+Abort.
+
+Lemma valid_glookup {P} {pred_P : PredicativeSig P} : forall {Δ x A},
+    {{ GC Δ ≈ Δ ∈ per_gctx pred_P }} ->
+    {{ `#x : A ∈ Δ }} ->
+    exists elem_rel,
+      rel_typ_unsorted pred_P Δ A d{{{ ⋅ }}} A d{{{ ⋅ }}} elem_rel /\ rel_exp Δ {{{ `#x }}} d{{{ ⋅ }}} {{{ `#x }}} d{{{ ⋅ }}} elem_rel.
+Proof.
+  intros * HΔΔ'.
+  gen x A.
+  induction HΔΔ'; intros * HxinΔ;
+    inversion HxinΔ; subst.
+
+    
+(** ** Cases for local variables *)
+Lemma valid_lookup {P : PtsSig} {pred_P : PredicativeSig P} : forall {Δ Γ x A env_relΓ}
+                        (equiv_Γ_Γ : {{ EF Γ ≈ Γ ∈ per_ctx_env pred_P Δ ↘ env_relΓ }}),
     {{ #x : A ∈ Γ }} ->
     forall ρ ρ' (equiv_p_p' : {{ Dom ρ ≈ ρ' ∈ env_relΓ }}),
     exists elem_rel,
-      rel_typ_unsorted pred_P A ρ A ρ' elem_rel /\ rel_exp {{{ #x }}} ρ {{{ #x }}} ρ' elem_rel.
+      rel_typ_unsorted pred_P Δ A ρ A ρ' elem_rel /\ rel_exp Δ {{{ #x }}} ρ {{{ #x }}} ρ' elem_rel.
 Proof with solve [split; mauto].
   intros * ? HxinΓ.
   assert {{ #x : A ∈ Γ }} as HxinΓ' by mauto.
-  remember Γ as Δ eqn:HΔΓ in HxinΓ', equiv_Γ_Γ at 2. clear HΔΓ. rename equiv_Γ_Γ into equiv_Γ_Δ.
+  remember Γ as Γ' eqn:HΓ'Γ in HxinΓ', equiv_Γ_Γ at 2. clear HΓ'Γ. rename equiv_Γ_Γ into equiv_Γ_Γ'.
   remember A as A' eqn:HAA' in HxinΓ' |- * at 2. clear HAA'.
-  gen Δ A' env_relΓ.
+  gen Γ' A' env_relΓ.
 
-  induction HxinΓ; intros * equiv_Γ_Δ HxinΓ0; inversion HxinΓ0; subst; clear HxinΓ0; inversion_clear equiv_Γ_Δ; subst; apply_relation_equivalence.
+  induction HxinΓ; intros * equiv_Γ_Γ' HxinΓ0; inversion HxinΓ0; subst; clear HxinΓ0; inversion_clear equiv_Γ_Γ'; subst; apply_relation_equivalence.
   - intros ? ? [];
       (on_all_hyp: destruct_rel_by_assumption tail_rel); destruct_conjs.
     simplify_evals.
@@ -27,12 +54,12 @@ Proof with solve [split; mauto].
     split; econstructor; mauto 3.
 
   - intros ? ? [].
-    specialize (IHHxinΓ _ _ _ equiv_Γ_Γ' H0 d{{{ ρ0 ↯ }}} d{{{ ρ'0 ↯ }}} equiv_ρ_drop_ρ'_drop).
+    specialize (IHHxinΓ _ _ _ equiv_Γ_Γ'0 H0 d{{{ ρ0 ↯ }}} d{{{ ρ'0 ↯ }}} equiv_ρ_drop_ρ'_drop).
     destruct_conjs.
     (on_all_hyp: destruct_rel_by_assumption tail_rel); destruct_conjs;
     eexists.
 
-    assert (rel_typ_unsorted pred_P B d{{{ ρ0 ↯ }}} B0 d{{{ ρ'0 ↯ }}} (head_rel d{{{ ρ0 ↯ }}} d{{{ ρ'0 ↯ }}} equiv_ρ_drop_ρ'_drop)) by mauto.
+    assert (rel_typ_unsorted pred_P Δ B d{{{ ρ0 ↯ }}} B0 d{{{ ρ'0 ↯ }}} (head_rel d{{{ ρ0 ↯ }}} d{{{ ρ'0 ↯ }}} equiv_ρ_drop_ρ'_drop)) by mauto.
     destruct_by_head (@rel_typ_unsorted P).
     destruct_by_head (@rel_exp P).
     dir_inversion_by_head (@eval_exp P); subst.
@@ -40,10 +67,10 @@ Proof with solve [split; mauto].
     split; econstructor; mauto.
 Qed.
 
-Lemma valid_exp_var {P} {pred_P : PredicativeSig P} : forall {Γ x A},
-    {{ ⟪ pred_P ⟫ ⊨ Γ }} ->
+Lemma valid_exp_var {P} {pred_P : PredicativeSig P} : forall {Δ Γ x A},
+    {{ ⟪ pred_P ⟫ Δ ▶ Γ }} ->
     {{ # x : A ∈ Γ }} ->
-    {{ ⟪ pred_P ⟫ Γ ⊨u #x : A }}.
+    {{ ⟪ pred_P ⟫ Δ ▶ Γ ⊨u #x : A }}.
 Proof.
   intros * [? equiv_Γ] Hx.
   eexists; split; [eassumption|].
@@ -54,21 +81,21 @@ Qed.
 #[export]
 Hint Resolve valid_exp_var : mcpts.
 
-Lemma rel_exp_var {P} {pred_P : PredicativeSig P} : forall {Γ x A},
-    {{ ⟪ pred_P ⟫ ⊨ Γ }} ->
+Lemma rel_exp_var {P} {pred_P : PredicativeSig P} : forall {Δ Γ x A},
+    {{ ⟪ pred_P ⟫ Δ ▶ Γ }} ->
     {{ # x : A ∈ Γ }} ->
-    {{ ⟪ pred_P ⟫ Γ ⊨u #x ≈ #x : A}}.
+    {{ ⟪ pred_P ⟫ Δ ▶ Γ ⊨u #x ≈ #x : A}}.
 Proof.
   intros.
   eapply valid_exp_var; mauto.
 Qed.
 
-Lemma rel_exp_var_0_sub {P} {pred_P : PredicativeSig P} : forall {Γ M σ Δ A},
-  {{ ⟪ pred_P ⟫ Γ ⊨s σ : Δ }} ->
-  {{ ⟪ pred_P ⟫ Γ ⊨u M : A[σ] }} ->
-  {{ ⟪ pred_P ⟫ Γ ⊨u #0[σ ,, M] ≈ M : A[σ] }}.
+Lemma rel_exp_var_0_sub {P} {pred_P : PredicativeSig P} : forall {Δ Γ M σ Γ' A},
+  {{ ⟪ pred_P ⟫ Δ ▶ Γ ⊨s σ : Γ' }} ->
+  {{ ⟪ pred_P ⟫ Δ ▶ Γ ⊨u M : A[σ] }} ->
+  {{ ⟪ pred_P ⟫ Δ ▶ Γ ⊨u #0[σ ,, M] ≈ M : A[σ] }}.
 Proof with mautosolve.
-  intros * [env_relΓ [? [env_relΔ]]] HM.
+  intros * [env_relΓ [? [env_relΓ']]] HM.
   invert_rel_exp_unsorted HM.
   destruct_conjs.
   eexists; split; [eassumption|].
@@ -85,13 +112,13 @@ Qed.
 #[export]
 Hint Resolve rel_exp_var_0_sub : mcpts.
 
-Lemma rel_exp_var_S_sub {P} {pred_P : PredicativeSig P} : forall {Γ M σ Δ A x B},
-  {{ ⟪ pred_P ⟫ Γ ⊨s σ : Δ }} ->
-  {{ ⟪ pred_P ⟫ Γ ⊨u M : A[σ] }} ->
-  {{ #x : B ∈ Δ }} ->
-  {{ ⟪ pred_P ⟫ Γ ⊨u #(S x)[σ ,, M] ≈ #x[σ] : B[σ] }}.
+Lemma rel_exp_var_S_sub {P} {pred_P : PredicativeSig P} : forall {Δ Γ M σ Γ' A x B},
+  {{ ⟪ pred_P ⟫ Δ ▶ Γ ⊨s σ : Γ' }} ->
+  {{ ⟪ pred_P ⟫ Δ ▶ Γ ⊨u M : A[σ] }} ->
+  {{ #x : B ∈ Γ' }} ->
+  {{ ⟪ pred_P ⟫ Δ ▶ Γ ⊨u #(S x)[σ ,, M] ≈ #x[σ] : B[σ] }}.
 Proof with mautosolve.
-  intros * [env_relΓ [? [env_relΔ]]] HM HxinΓ.
+  intros * [env_relΓ [? [env_relΓ']]] HM HxinΓ.
   invert_rel_exp_unsorted HM.
   destruct_conjs.
   pose proof (valid_lookup ltac:(eassumption) HxinΓ).
@@ -99,9 +126,8 @@ Proof with mautosolve.
   eexists; split; [eassumption|].
   intros.
   (on_all_hyp: destruct_rel_by_assumption env_relΓ).
-  (on_all_hyp: destruct_rel_by_assumption env_relΔ).
+  (on_all_hyp: destruct_rel_by_assumption env_relΓ').
   destruct_by_head (@rel_typ_unsorted P).
-  destruct_by_head (@rel_typ P).
   destruct_by_head (@rel_exp P).
   dir_inversion_by_head (@eval_exp P); subst.
   functional_eval_rewrite_clear.
@@ -113,10 +139,10 @@ Qed.
 #[export]
 Hint Resolve rel_exp_var_S_sub : mcpts.
 
-Lemma rel_exp_var_weaken {P} {pred_P : PredicativeSig P} : forall {Γ B x A},
-    {{ ⟪ pred_P ⟫ ⊨ Γ, B }} ->
+Lemma rel_exp_var_weaken {P} {pred_P : PredicativeSig P} : forall {Δ Γ B x A},
+    {{ ⟪ pred_P ⟫ Δ ▶ Γ, B }} ->
     {{ #x : A ∈ Γ }} ->
-    {{ ⟪ pred_P ⟫ Γ, B ⊨u #x[Wk] ≈ #(S x) : A[Wk] }}.
+    {{ ⟪ pred_P ⟫ Δ ▶ Γ, B ⊨u #x[Wk] ≈ #(S x) : A[Wk] }}.
 Proof with mautosolve.
   intros * [env_relΓB] HxinΓ.
   invert_per_ctx_envs_unsorted.
@@ -128,7 +154,6 @@ Proof with mautosolve.
   destruct_by_head (@cons_per_ctx_env P).
   rename tail_rel into env_relΓ.
   (on_all_hyp: destruct_rel_by_assumption env_relΓ).
-  destruct_by_head (@rel_typ P).
   destruct_by_head (@rel_typ_unsorted P).
   destruct_by_head (@rel_exp P).
   dir_inversion_by_head (@eval_exp P); subst.
