theories/Core/Semantic/PER/Lemmas.v
@@ -1957,3 +1957,79 @@ Proof.
   inversion H; subst.
   eexists; reflexivity.
 Qed.
+
+
+(** ** Weakening of global contexts in PER model *)
+Lemma gctx_weaken_per_bot {P} : forall {Δ : gctx P} {e e' x B},
+    {{ Dom e ≈ e' ∈ per_bot Δ }} ->
+    {{ `#x ∉ Δ }} ->
+    {{ Dom e ≈ e' ∈ per_bot ((x, B) :: Δ) }}.
+Proof.
+  intros * Hbot Hfresh i;
+    specialize (Hbot i) as [E []];
+    repeat eexists; mauto 2.
+Qed.
+
+Lemma gctx_weaken_per_top {P} : forall {Δ : gctx P} {w w' x B},
+    {{ Dom w ≈ w' ∈ per_top Δ }} ->
+    {{ `#x ∉ Δ }} ->
+    {{ Dom w ≈ w' ∈ per_top ((x, B) :: Δ) }}.
+Proof.
+  intros * Htop Hfresh i;
+    specialize (Htop i) as [W []];
+    repeat eexists; mauto 2.
+Qed.
+
+Lemma gctx_weaken_per_top_typ {P} : forall {Δ : gctx P} {a a' x B},
+    {{ Dom a ≈ a' ∈ per_top_typ Δ }} ->
+    {{ `#x ∉ Δ }} ->
+    {{ Dom a ≈ a' ∈ per_top_typ ((x, B) :: Δ) }}.
+Proof.
+  intros * Htop_typ Hfresh i;
+    specialize (Htop_typ i) as [A []];
+    repeat eexists; mauto 2.
+Qed.
+
+#[export]
+Hint Resolve gctx_weaken_per_bot gctx_weaken_per_top gctx_weaken_per_top_typ : mcpts.
+ 
+Lemma gctx_weaken_per_nat {P} : forall {Δ : gctx P} {n n' x B},
+    {{ Dom n ≈ n' ∈ per_nat Δ }} ->
+    {{ `#x ∉ Δ }} ->
+    {{ Dom n ≈ n' ∈ per_nat ((x, B) :: Δ) }}.
+Proof.
+  induction 1; intros; mauto 3.
+Qed.
+
+#[export]
+Hint Resolve gctx_weaken_per_nat : mcpts.
+
+Lemma gctx_weaken_per_ne {P} : forall {Δ : gctx P} {m m' x B},
+    {{ Dom m ≈ m' ∈ per_ne Δ }} ->
+    {{ `#x ∉ Δ }} ->
+    {{ Dom m ≈ m' ∈ per_ne ((x, B) :: Δ) }}.
+Proof.
+  induction 1; intros; mauto 3.
+Qed.
+
+#[export]
+Hint Resolve gctx_weaken_per_ne : mcpts.
+
+Lemma gctx_weaken_per_sort_elem {P} {pred_P : PredicativeSig P} : forall {Δ : gctx P} {x B a a' s R},
+    {{ `#x ∉ Δ }} ->
+    {{ DF a ≈ a' ∈ per_sort_elem pred_P Δ s ↘ R }} ->
+    exists R',
+      {{ DF a ≈ a' ∈ per_sort_elem pred_P ((x, B) :: Δ) s ↘ R' }}.
+Proof.
+  simpl.
+  intros * Hfresh.
+  induction 1 using per_sort_elem_ind.
+  - eexists; (unshelve per_sort_elem_econstructor; mauto 2).
+    reflexivity.
+  - destruct IHper_sort_elem as [in_rel'].
+    admit.
+  - eexists; per_sort_elem_econstructor; mauto 2.
+    reflexivity.
+  - eexists; per_sort_elem_econstructor; mauto 2.
+    reflexivity.
+      
